<?xml version="1.0"?>
<rdf:RDF xmlns="https://purl.org/vir/"
     xml:base="https://purl.org/vir/"
     xmlns:owl="http://www.w3.org/2002/07/owl#"
     xmlns:rdf="http://www.w3.org/1999/02/22-rdf-syntax-ns#"
     xmlns:xml="http://www.w3.org/XML/1998/namespace"
     xmlns:xsd="http://www.w3.org/2001/XMLSchema#"
     xmlns:dc="http://purl.org/dc/elements/1.1/"
     xmlns:rdfs="http://www.w3.org/2000/01/rdf-schema#">
    <owl:Ontology rdf:about="https://purl.org/vir/">
        <rdfs:comment>An extension of CIDOC-CRM to support propositions about visual items. With the term visual items we refers to those signs, present in 2D/3D representations, which are identified as having their own identity.</rdfs:comment>
        <rdfs:label xml:lang="en">VIsual Representation</rdfs:label>
        <owl:versionInfo>0.4</owl:versionInfo>
        <dc:creator>Nicola Carboni</dc:creator>
    </owl:Ontology>
    


    <!-- 
    ///////////////////////////////////////////////////////////////////////////////////////
    //
    // Object Properties
    //
    ///////////////////////////////////////////////////////////////////////////////////////
     -->

    





    <!-- https://purl.org/vir/K10_on_the_base_of -->

    <owl:ObjectProperty rdf:about="https://purl.org/vir/K10_on_the_base_of">
        <rdfs:subPropertyOf rdf:resource="http://www.cidoc-crm.org/cidoc-crm/P16_used_specific_object"/>
        <owl:inverseOf rdf:resource="https://purl.org/vir/K10i_is_basis_for"/>
        <rdfs:comment>The property describes the source used for the status assignment</rdfs:comment>
        <rdfs:label xml:lang="en">On the base of</rdfs:label>
    </owl:ObjectProperty>
    


    <!-- https://purl.org/vir/K10i_is_basis_for -->

    <owl:ObjectProperty rdf:about="https://purl.org/vir/K10i_is_basis_for">
        <rdfs:subPropertyOf rdf:resource="http://www.cidoc-crm.org/cidoc-crm/P16i_was_used_for"/>
        <rdfs:domain rdf:resource="http://www.cidoc-crm.org/cidoc-crm/E89_Propositional_Object"/>
        <rdfs:comment>The property describes the source used for the status assignment</rdfs:comment>
        <rdfs:label xml:lang="en">is based on</rdfs:label>
    </owl:ObjectProperty>
    


    <!-- https://purl.org/vir/K11_assigned -->

    <owl:ObjectProperty rdf:about="https://purl.org/vir/K11_assigned">
        <rdfs:subPropertyOf rdf:resource="http://www.cidoc-crm.org/cidoc-crm/P141_assigned"/>
        <owl:inverseOf rdf:resource="https://purl.org/vir/K11i_was_assigned_by"/>
        <rdfs:domain rdf:resource="https://purl.org/vir/IC12_Visual_Recognition"/>
        <rdfs:range rdf:resource="https://purl.org/vir/IC9_Iconographical_Object"/>
        <rdfs:comment>The property indicates the status assigned during the visual recognition event</rdfs:comment>
        <rdfs:label xml:lang="en">assigned</rdfs:label>
    </owl:ObjectProperty>
    


    <!-- https://purl.org/vir/K11i_was_assigned_by -->

    <owl:ObjectProperty rdf:about="https://purl.org/vir/K11i_was_assigned_by">
        <rdfs:subPropertyOf rdf:resource="http://www.cidoc-crm.org/cidoc-crm/P141i_was_assigned_by"/>
        <rdfs:domain rdf:resource="https://purl.org/vir/IC9_Iconographical_Object"/>
        <rdfs:range rdf:resource="https://purl.org/vir/IC12_Visual_Recognition"/>
        <rdfs:comment xml:lang="en">The property indicates the status assigned during the visual recognition event</rdfs:comment>
        <rdfs:label xml:lang="en">was assigned by</rdfs:label>
    </owl:ObjectProperty>
    


    <!-- https://purl.org/vir/K14_has_theme -->

    <owl:ObjectProperty rdf:about="https://purl.org/vir/K14_has_theme">
        <rdfs:subPropertyOf rdf:resource="http://www.cidoc-crm.org/cidoc-crm/P2_has_type"/>
        <owl:inverseOf rdf:resource="https://purl.org/vir/K14i_is_theme_of"/>
        <rdfs:domain rdf:resource="http://www.cidoc-crm.org/cidoc-crm/E36_Visual_Item"/>
        <rdfs:comment>The property document a theme, chosen from a vocabulary, assigned to a specific iconographical object</rdfs:comment>
        <rdfs:label xml:lang="en">has theme</rdfs:label>
    </owl:ObjectProperty>
    


    <!-- https://purl.org/vir/K14i_is_theme_of -->

    <owl:ObjectProperty rdf:about="https://purl.org/vir/K14i_is_theme_of">
        <rdfs:subPropertyOf rdf:resource="http://www.cidoc-crm.org/cidoc-crm/P2i_is_type_of"/>
        <rdfs:domain rdf:resource="http://www.cidoc-crm.org/cidoc-crm/E55_Type"/>
        <rdfs:comment>The property document a theme, chosen from a vocabulary, assigned to a specific iconographical object</rdfs:comment>
        <rdfs:label xml:lang="en">is theme of</rdfs:label>
    </owl:ObjectProperty>
    


    <!-- https://purl.org/vir/K17_has_attribute -->

    <owl:ObjectProperty rdf:about="https://purl.org/vir/K17_has_attribute">
        <rdfs:subPropertyOf rdf:resource="http://www.cidoc-crm.org/cidoc-crm/P106_is_composed_of"/>
        <owl:inverseOf rdf:resource="https://purl.org/vir/K17i_is_attribute_of"/>
        <rdfs:domain rdf:resource="https://purl.org/vir/IC9_Iconographical_Object"/>
        <rdfs:range rdf:resource="https://purl.org/vir/IC10_Iconographical_Attribute"/>
        <rdfs:comment xml:lang="en">This property associates an attribute with the iconographical object where it is depicted</rdfs:comment>
        <rdfs:label xml:lang="en">has attribute</rdfs:label>
    </owl:ObjectProperty>
    


    <!-- https://purl.org/vir/K17i_is_attribute_of -->

    <owl:ObjectProperty rdf:about="https://purl.org/vir/K17i_is_attribute_of">
        <rdfs:subPropertyOf rdf:resource="http://www.cidoc-crm.org/cidoc-crm/P106i_forms_part_of"/>
        <rdfs:domain rdf:resource="https://purl.org/vir/IC10_Iconographical_Attribute"/>
        <rdfs:range rdf:resource="https://purl.org/vir/IC9_Iconographical_Object"/>
        <rdfs:comment xml:lang="en">This property associates an attribute with the iconographical object where it is depicted</rdfs:comment>
        <rdfs:label xml:lang="en">is attribute of</rdfs:label>
    </owl:ObjectProperty>
    


    <!-- https://purl.org/vir/K1_denotes -->

    <owl:ObjectProperty rdf:about="https://purl.org/vir/K1_denotes">
        <rdfs:subPropertyOf rdf:resource="http://www.cidoc-crm.org/cidoc-crm/P65_shows_visual_item"/>
        <owl:inverseOf rdf:resource="https://purl.org/vir/K1i_is_denoted_by"/>
        <rdfs:domain rdf:resource="https://purl.org/vir/IC1_Iconographical_Atom"/>
        <rdfs:range rdf:resource="http://www.cidoc-crm.org/cidoc-crm/E36_Visual_Item"/>
        <rdfs:comment>The property document the assignment of an iconographical object to a specific physical man-made object</rdfs:comment>
        <rdfs:label xml:lang="en">Denote</rdfs:label>
    </owl:ObjectProperty>
    


    <!-- https://purl.org/vir/K1i_is_denoted_by -->

    <owl:ObjectProperty rdf:about="https://purl.org/vir/K1i_is_denoted_by">
        <rdfs:subPropertyOf rdf:resource="http://www.cidoc-crm.org/cidoc-crm/P65i_is_shown_by"/>
        <rdfs:domain rdf:resource="http://www.cidoc-crm.org/cidoc-crm/E36_Visual_Item"/>
        <rdfs:range rdf:resource="https://purl.org/vir/IC1_Iconographical_Atom"/>
        <rdfs:comment xml:lang="en">The property document the assignment of an iconographical object to a specific physical man-made object</rdfs:comment>
        <rdfs:label xml:lang="en">is denoted by</rdfs:label>
    </owl:ObjectProperty>
    


    <!-- https://purl.org/vir/K20_forms_part_of -->

    <owl:ObjectProperty rdf:about="https://purl.org/vir/K20_forms_part_of">
        <rdfs:subPropertyOf rdf:resource="http://www.cidoc-crm.org/cidoc-crm/P148_has_component"/>
        <owl:inverseOf rdf:resource="https://purl.org/vir/K20i_is_composed_of"/>
        <rdfs:domain rdf:resource="https://purl.org/vir/IC9_Iconographical_Object"/>
        <rdfs:range rdf:resource="https://purl.org/vir/IC9_Iconographical_Object"/>
        <rdfs:comment xml:lang="en">This property put in relation an iconographical object with a part of itself.</rdfs:comment>
        <rdfs:label xml:lang="en">forms part of</rdfs:label>
    </owl:ObjectProperty>
    


    <!-- https://purl.org/vir/K20i_is_composed_of -->

    <owl:ObjectProperty rdf:about="https://purl.org/vir/K20i_is_composed_of">
        <rdfs:subPropertyOf rdf:resource="http://www.cidoc-crm.org/cidoc-crm/P148i_is_component_of"/>
        <rdfs:domain rdf:resource="https://purl.org/vir/IC9_Iconographical_Object"/>
        <rdfs:range rdf:resource="https://purl.org/vir/IC9_Iconographical_Object"/>
        <rdfs:comment>This property put in relation an iconographical object with a part of itself.</rdfs:comment>
        <rdfs:label xml:lang="en">is composed of</rdfs:label>
    </owl:ObjectProperty>
    


    <!-- https://purl.org/vir/K21_depict -->

    <owl:ObjectProperty rdf:about="https://purl.org/vir/K21_depict">
        <rdfs:subPropertyOf rdf:resource="http://www.cidoc-crm.org/cidoc-crm/P138_represents"/>
        <owl:inverseOf rdf:resource="https://purl.org/vir/K21i_is_depiction_of_attribute"/>
        <rdfs:domain rdf:resource="https://purl.org/vir/IC10_Iconographical_Attribute"/>
        <rdfs:range rdf:resource="http://www.cidoc-crm.org/cidoc-crm/E70_Thing"/>
        <rdfs:comment xml:lang="em">This property indicates the entity referred by the rvisual epresentation</rdfs:comment>
        <rdfs:label xml:lang="en">depict</rdfs:label>
    </owl:ObjectProperty>
    


    <!-- https://purl.org/vir/K21i_is_depiction_of_attribute -->

    <owl:ObjectProperty rdf:about="https://purl.org/vir/K21i_is_depiction_of_attribute">
        <rdfs:subPropertyOf rdf:resource="http://www.cidoc-crm.org/cidoc-crm/P138i_has_representation"/>
        <rdfs:domain rdf:resource="http://www.cidoc-crm.org/cidoc-crm/E70_Thing"/>
        <rdfs:range rdf:resource="https://purl.org/vir/IC10_Iconographical_Attribute"/>
        <rdfs:comment>This property indicates the entity referred by the rvisual epresentation</rdfs:comment>
        <rdfs:label xml:lang="en">is depiction of attribute</rdfs:label>
    </owl:ObjectProperty>
    


    <!-- https://purl.org/vir/K22_has_personification -->

    <owl:ObjectProperty rdf:about="https://purl.org/vir/K22_has_personification">
        <rdfs:subPropertyOf rdf:resource="http://www.cidoc-crm.org/cidoc-crm/P138_represents"/>
        <owl:inverseOf rdf:resource="https://purl.org/vir/K22i_is_present_in"/>
        <rdfs:domain rdf:resource="https://purl.org/vir/IC9_Iconographical_Object"/>
        <rdfs:range rdf:resource="https://purl.org/vir/IC11_Personification"/>
        <rdfs:comment>This property indicates the membership of a personification in an iconographical object</rdfs:comment>
        <rdfs:label xml:lang="en">has personification</rdfs:label>
    </owl:ObjectProperty>
    


    <!-- https://purl.org/vir/K22i_is_present_in -->

    <owl:ObjectProperty rdf:about="https://purl.org/vir/K22i_is_present_in">
        <rdfs:subPropertyOf rdf:resource="http://www.cidoc-crm.org/cidoc-crm/P138i_has_representation"/>
        <rdfs:domain rdf:resource="https://purl.org/vir/IC16_Character"/>
        <rdfs:range rdf:resource="https://purl.org/vir/IC9_Iconographical_Object"/>
        <rdfs:comment>This property indicates the membership of a personification in an iconographical object</rdfs:comment>
        <rdfs:label xml:lang="en">is present in</rdfs:label>
    </owl:ObjectProperty>
    


    <!-- https://purl.org/vir/K23_connote -->

    <owl:ObjectProperty rdf:about="https://purl.org/vir/K23_connote">
        <rdfs:subPropertyOf rdf:resource="http://www.cidoc-crm.org/cidoc-crm/P138_represents"/>
        <owl:inverseOf rdf:resource="https://purl.org/vir/K23i_is_connotation_of"/>
        <rdfs:domain rdf:resource="https://purl.org/vir/IC9_Iconographical_Object"/>
        <rdfs:range rdf:resource="http://www.cidoc-crm.org/cidoc-crm/E28_Conceptual_Object"/>
        <rdfs:comment>This property indicates the connotation relationships, formalised by Barthes, between a conceptual entity and an iconographical object</rdfs:comment>
        <rdfs:label xml:lang="en">connote</rdfs:label>
    </owl:ObjectProperty>
    


    <!-- https://purl.org/vir/K23i_is_connotation_of -->

    <owl:ObjectProperty rdf:about="https://purl.org/vir/K23i_is_connotation_of">
        <rdfs:subPropertyOf rdf:resource="http://www.cidoc-crm.org/cidoc-crm/P138i_has_representation"/>
        <rdfs:domain rdf:resource="http://www.cidoc-crm.org/cidoc-crm/E28_Conceptual_Object"/>
        <rdfs:range rdf:resource="https://purl.org/vir/IC9_Iconographical_Object"/>
        <rdfs:comment>This property indicates the connotation relationships, formalised by Barthes, between a conceptual entity and an iconographical object.</rdfs:comment>
        <rdfs:label xml:lang="en">is connoted by</rdfs:label>
    </owl:ObjectProperty>
    


    <!-- https://purl.org/vir/K24_portray -->

    <owl:ObjectProperty rdf:about="https://purl.org/vir/K24_portray">
        <rdfs:subPropertyOf rdf:resource="http://www.cidoc-crm.org/cidoc-crm/P138_represents"/>
        <owl:inverseOf rdf:resource="https://purl.org/vir/K24i_is_portrayed_in"/>
        <rdfs:domain rdf:resource="https://purl.org/vir/IC9_Iconographical_Object"/>
        <rdfs:range rdf:resource="https://purl.org/vir/IC16_Character"/>
        <rdfs:comment xml:lang="en">This property put in relation an iconographical object with the portrayed character.</rdfs:comment>
        <rdfs:label xml:lang="en">portray</rdfs:label>
    </owl:ObjectProperty>
    


    <!-- https://purl.org/vir/K24i_is_portrayed_in -->

    <owl:ObjectProperty rdf:about="https://purl.org/vir/K24i_is_portrayed_in">
        <rdfs:subPropertyOf rdf:resource="http://www.cidoc-crm.org/cidoc-crm/P138i_has_representation"/>
        <rdfs:domain rdf:resource="https://purl.org/vir/IC16_Character"/>
        <rdfs:range rdf:resource="https://purl.org/vir/IC9_Iconographical_Object"/>
        <rdfs:comment xml:lang="en">This property put in relation an iconographical object with the portrayed character.</rdfs:comment>
        <rdfs:label xml:lang="en">is portrayed by</rdfs:label>
    </owl:ObjectProperty>
    


    <!-- https://purl.org/vir/K25_symbolize -->

    <owl:ObjectProperty rdf:about="https://purl.org/vir/K25_symbolize">
        <rdfs:subPropertyOf rdf:resource="http://www.cidoc-crm.org/cidoc-crm/P138_represents"/>
        <owl:inverseOf rdf:resource="https://purl.org/vir/K25i_is_personification_of"/>
        <rdfs:domain rdf:resource="https://purl.org/vir/IC11_Personification"/>
        <rdfs:range rdf:resource="http://www.cidoc-crm.org/cidoc-crm/E28_Conceptual_Object"/>
        <rdfs:comment xml:lang="en">This property put in relation a conceptual object with its personification in a work of art</rdfs:comment>
        <rdfs:label xml:lang="en">symbolize</rdfs:label>
    </owl:ObjectProperty>
    


    <!-- https://purl.org/vir/K25i_is_personification_of -->

    <owl:ObjectProperty rdf:about="https://purl.org/vir/K25i_is_personification_of">
        <rdfs:subPropertyOf rdf:resource="http://www.cidoc-crm.org/cidoc-crm/P138i_has_representation"/>
        <rdfs:domain rdf:resource="http://www.cidoc-crm.org/cidoc-crm/E28_Conceptual_Object"/>
        <rdfs:range rdf:resource="https://purl.org/vir/IC11_Personification"/>
        <rdfs:comment>This property put in relation a conceptual object with its personification in a work of art</rdfs:comment>
        <rdfs:label xml:lang="en">is personification of</rdfs:label>
    </owl:ObjectProperty>
    


    <!-- https://purl.org/vir/K27_rest_on -->

    <owl:ObjectProperty rdf:about="https://purl.org/vir/K27_rest_on">
        <rdfs:subPropertyOf rdf:resource="http://www.cidoc-crm.org/cidoc-crm/P56i_is_found_on"/>
        <owl:inverseOf rdf:resource="https://purl.org/vir/K27i_has_layer"/>
        <rdfs:domain rdf:resource="https://purl.org/vir/IC8_Layer"/>
        <rdfs:comment xml:lang="en">This property associates an instance of S8 Layer with the Physical Thing it rest on</rdfs:comment>
        <rdfs:label xml:lang="en">rest on</rdfs:label>
    </owl:ObjectProperty>
    


    <!-- https://purl.org/vir/K27i_has_layer -->

    <owl:ObjectProperty rdf:about="https://purl.org/vir/K27i_has_layer">
        <rdfs:subPropertyOf rdf:resource="http://www.cidoc-crm.org/cidoc-crm/P56_bears_feature"/>
        <rdfs:comment>This property associates an instance of S8 Layer with the Physical Thing it rest on</rdfs:comment>
        <rdfs:label xml:lang="en">has layer</rdfs:label>
    </owl:ObjectProperty>
    


    <!-- https://purl.org/vir/K34_illustrate -->

    <owl:ObjectProperty rdf:about="https://purl.org/vir/K34_illustrate">
        <rdfs:subPropertyOf rdf:resource="http://www.cidoc-crm.org/cidoc-crm/P138_represents"/>
        <owl:inverseOf rdf:resource="https://purl.org/vir/K34i_is_illustrated_by"/>
        <rdfs:domain rdf:resource="https://purl.org/vir/IC9_Iconographical_Object"/>
        <rdfs:range rdf:resource="http://www.cidoc-crm.org/cidoc-crm/E73_Information_Object"/>
        <rdfs:comment>This property associate an information object to a iconographical representation</rdfs:comment>
        <rdfs:label xml:lang="en">illustrate</rdfs:label>
    </owl:ObjectProperty>
    


    <!-- https://purl.org/vir/K34i_is_illustrated_by -->

    <owl:ObjectProperty rdf:about="https://purl.org/vir/K34i_is_illustrated_by">
        <rdfs:subPropertyOf rdf:resource="http://www.cidoc-crm.org/cidoc-crm/P138i_has_representation"/>
        <rdfs:domain rdf:resource="http://www.cidoc-crm.org/cidoc-crm/E73_Information_Object"/>
        <rdfs:range rdf:resource="https://purl.org/vir/IC9_Iconographical_Object"/>
        <rdfs:comment>This property associate an information object to a iconographical representation</rdfs:comment>
        <rdfs:label xml:lang="en">is illustrated by</rdfs:label>
    </owl:ObjectProperty>
    


    <!-- https://purl.org/vir/K36_anchors -->

    <owl:ObjectProperty rdf:about="https://purl.org/vir/K36_anchors">
        <rdfs:subPropertyOf rdf:resource="http://www.cidoc-crm.org/cidoc-crm/P141_assigned"/>
        <owl:inverseOf rdf:resource="https://purl.org/vir/K36i_was_anchored_by"/>
        <rdfs:domain rdf:resource="https://purl.org/vir/IC17_Anchorage"/>
        <rdfs:range rdf:resource="http://www.cidoc-crm.org/cidoc-crm/E28_Conceptual_Object"/>
        <rdfs:label xml:lang="en">anchors</rdfs:label>
    </owl:ObjectProperty>
    


    <!-- https://purl.org/vir/K36i_was_anchored_by -->

    <owl:ObjectProperty rdf:about="https://purl.org/vir/K36i_was_anchored_by">
        <rdfs:subPropertyOf rdf:resource="http://www.cidoc-crm.org/cidoc-crm/P141i_was_assigned_by"/>
        <rdfs:domain rdf:resource="http://www.cidoc-crm.org/cidoc-crm/E28_Conceptual_Object"/>
        <rdfs:range rdf:resource="https://purl.org/vir/IC17_Anchorage"/>
        <rdfs:label xml:lang="en">was anchored by</rdfs:label>
    </owl:ObjectProperty>
    


    <!-- https://purl.org/vir/K37_anchors_to -->

    <owl:ObjectProperty rdf:about="https://purl.org/vir/K37_anchors_to">
        <rdfs:subPropertyOf rdf:resource="http://www.cidoc-crm.org/cidoc-crm/P141_assigned"/>
        <owl:inverseOf rdf:resource="https://purl.org/vir/K37i_is_anchored_by"/>
        <rdfs:domain rdf:resource="https://purl.org/vir/IC17_Anchorage"/>
        <rdfs:range rdf:resource="http://www.cidoc-crm.org/cidoc-crm/E36_Visual_Item"/>
        <rdfs:label xml:lang="en">anchors to</rdfs:label>
    </owl:ObjectProperty>
    


    <!-- https://purl.org/vir/K37i_is_anchored_by -->

    <owl:ObjectProperty rdf:about="https://purl.org/vir/K37i_is_anchored_by">
        <rdfs:subPropertyOf rdf:resource="http://www.cidoc-crm.org/cidoc-crm/P141i_was_assigned_by"/>
        <rdfs:domain rdf:resource="http://www.cidoc-crm.org/cidoc-crm/E36_Visual_Item"/>
        <rdfs:range rdf:resource="https://purl.org/vir/IC17_Anchorage"/>
        <rdfs:label xml:lang="en">is anchored by</rdfs:label>
    </owl:ObjectProperty>
    


    <!-- https://purl.org/vir/K38_observed_colour -->

    <owl:ObjectProperty rdf:about="https://purl.org/vir/K38_observed_colour">
        <rdfs:subPropertyOf rdf:resource="http://www.ics.forth.gr/isl/CRMsci/O9_observed_property_type"/>
        <owl:inverseOf rdf:resource="https://purl.org/vir/K38i_has_been_obvserved_in"/>
        <rdfs:domain rdf:resource="https://purl.org/vir/IC12_Visual_Recognition"/>
        <rdfs:range rdf:resource="https://purl.org/vir/IC5_Color"/>
        <rdfs:comment></rdfs:comment>
        <rdfs:label xml:lang="en">observed colour</rdfs:label>
    </owl:ObjectProperty>
    


    <!-- https://purl.org/vir/K38i_has_been_obvserved_in -->

    <owl:ObjectProperty rdf:about="https://purl.org/vir/K38i_has_been_obvserved_in">
        <rdfs:subPropertyOf rdf:resource="http://www.ics.forth.gr/isl/CRMsci/O9i_property_type_was_observed_by"/>
        <rdfs:domain rdf:resource="https://purl.org/vir/IC5_Color"/>
        <rdfs:range rdf:resource="https://purl.org/vir/IC12_Visual_Recognition"/>
        <rdfs:label xml:lang="en">has been observed in</rdfs:label>
    </owl:ObjectProperty>
    


    <!-- https://purl.org/vir/K4_is_visual_prototype_of -->

    <owl:ObjectProperty rdf:about="https://purl.org/vir/K4_is_visual_prototype_of">
        <rdfs:subPropertyOf rdf:resource="http://www.cidoc-crm.org/cidoc-crm/P67_refers_to"/>
        <owl:inverseOf rdf:resource="https://purl.org/vir/K4i_has_visual_prototype"/>
        <rdfs:domain rdf:resource="https://purl.org/vir/IC9_Iconographical_Object"/>
        <rdfs:range rdf:resource="https://purl.org/vir/IC9_Iconographical_Object"/>
        <rdfs:comment>The property documents the use of a specific prototypical example for an image. The nature of the relationships helps define a map of relationships between prototypical items used in the arts.</rdfs:comment>
        <rdfs:label xml:lang="en">is visual prototype of</rdfs:label>
    </owl:ObjectProperty>
    


    <!-- https://purl.org/vir/K4i_has_visual_prototype -->

    <owl:ObjectProperty rdf:about="https://purl.org/vir/K4i_has_visual_prototype">
        <rdfs:subPropertyOf rdf:resource="http://www.cidoc-crm.org/cidoc-crm/P67i_is_referred_to_by"/>
        <rdfs:domain rdf:resource="https://purl.org/vir/IC9_Iconographical_Object"/>
        <rdfs:range rdf:resource="https://purl.org/vir/IC9_Iconographical_Object"/>
        <rdfs:comment>The property documents the use of a specific prototypical example for an image. The nature of the relationships helps define a map of relationships between prototypical items used in the arts.</rdfs:comment>
        <rdfs:label xml:lang="en">has visual prototype</rdfs:label>
    </owl:ObjectProperty>
    


    <!-- https://purl.org/vir/K9_Assigned_status_to -->

    <owl:ObjectProperty rdf:about="https://purl.org/vir/K9_Assigned_status_to">
        <rdfs:subPropertyOf rdf:resource="http://www.cidoc-crm.org/cidoc-crm/P140_assigned_attribute_to"/>
        <owl:inverseOf rdf:resource="https://purl.org/vir/K9i_has_status_assigned_by"/>
        <rdfs:domain rdf:resource="https://purl.org/vir/IC12_Visual_Recognition"/>
        <rdfs:range rdf:resource="http://www.cidoc-crm.org/cidoc-crm/E18_Physical_Thing"/>
        <rdfs:comment xml:lang="en">The property documents the assignment of status to a specific physical thing</rdfs:comment>
        <rdfs:label xml:lang="en">Assigned status to</rdfs:label>
    </owl:ObjectProperty>
    


    <!-- https://purl.org/vir/K9i_has_status_assigned_by -->

    <owl:ObjectProperty rdf:about="https://purl.org/vir/K9i_has_status_assigned_by">
        <rdfs:subPropertyOf rdf:resource="http://www.cidoc-crm.org/cidoc-crm/P140i_was_attributed_by"/>
        <rdfs:domain rdf:resource="http://www.cidoc-crm.org/cidoc-crm/E18_Physical_Thing"/>
        <rdfs:range rdf:resource="https://purl.org/vir/IC12_Visual_Recognition"/>
        <rdfs:comment xml:lang="en">The property documents the assignment of status to a specific physical thing.</rdfs:comment>
        <rdfs:label xml:lang="en">has status assigned by</rdfs:label>
    </owl:ObjectProperty>
    


    <!-- 
    ///////////////////////////////////////////////////////////////////////////////////////
    //
    // Classes
    //
    ///////////////////////////////////////////////////////////////////////////////////////
     -->

    


    

    <!-- https://purl.org/vir/IC10_Iconographical_Attribute -->

    <owl:Class rdf:about="https://purl.org/vir/IC10_Iconographical_Attribute">
        <rdfs:subClassOf rdf:resource="http://www.cidoc-crm.org/cidoc-crm/E36_Visual_Item"/>
        <owl:disjointWith rdf:resource="https://purl.org/vir/IC9_Iconographical_Object"/>
        <rdfs:comment>An object that help identify and usually accompanied certain type of iconographic representation, and help define the character or a type of character portrayed. They usually are taken from on episode of the life of the character depicted</rdfs:comment>
        <rdfs:label xml:lang="en">Iconographical Attribute</rdfs:label>
    </owl:Class>
    


    <!-- https://purl.org/vir/IC11_Personification -->

    <owl:Class rdf:about="https://purl.org/vir/IC11_Personification">
        <rdfs:subClassOf rdf:resource="https://purl.org/vir/IC9_Iconographical_Object"/>
        <rdfs:comment>A human, or anthropomorphic figure, that represents an abstract idea or a concept</rdfs:comment>
        <rdfs:label xml:lang="en">Personification</rdfs:label>
    </owl:Class>
    


    <!-- https://purl.org/vir/IC12_Visual_Recognition -->

    <owl:Class rdf:about="https://purl.org/vir/IC12_Visual_Recognition">
        <rdfs:subClassOf rdf:resource="http://www.ics.forth.gr/isl/CRMsci/S4_Observation"/>
        <rdfs:comment xml:lang="en">The activity of assigning the iconographical status to a man-made object, or to one of its parts. It takes into account the possibility to link it to a speech act or a document where the authoritative proposition is clearly made</rdfs:comment>
        <rdfs:label xml:lang="en">Visual Recognition</rdfs:label>
    </owl:Class>
    


    <!-- https://purl.org/vir/IC16_Character -->

    <owl:Class rdf:about="https://purl.org/vir/IC16_Character">
        <rdfs:subClassOf rdf:resource="http://iflastandards.info/ns/fr/frbr/frbroo/F38_Character"/>
        <rdfs:comment>This class comprises fictional individuals, or groups, appearing in a 2D/3D representation. Each character portrayed can have a type, for example “Saint” or “layman”. Every saints portrayed is considered here as a character and not as an actor</rdfs:comment>
        <rdfs:label xml:lang="en">Character</rdfs:label>
    </owl:Class>
    


    <!-- https://purl.org/vir/IC17_Anchorage -->

    <owl:Class rdf:about="https://purl.org/vir/IC17_Anchorage">
        <rdfs:subClassOf rdf:resource="http://www.ics.forth.gr/isl/CRMsci/S4_Observation"/>
        <rdfs:comment>The class document the phenomenon of anchorage defined by Barthes as linguistic elements, which can serve to &apos;anchor&apos; (or constrain) to a specific readings of an image. Example can be inscription, which constrain a specific readings of an iconographical object, or the caption used for a photos.</rdfs:comment>
        <rdfs:label xml:lang="en">Anchorage</rdfs:label>
    </owl:Class>
    


    <!-- https://purl.org/vir/IC1_Iconographical_Atom -->

    <owl:Class rdf:about="https://purl.org/vir/IC1_Iconographical_Atom">
        <rdfs:subClassOf rdf:resource="http://www.cidoc-crm.org/cidoc-crm/E22_Man-Made_Object"/>
        <rdfs:comment>An Iconographical Atom is a physical arrangement of forms and colours created by human activity</rdfs:comment>
        <rdfs:label xml:lang="en">Iconographical Atom</rdfs:label>
    </owl:Class>
    


    <!-- https://purl.org/vir/IC5_Color -->

    <owl:Class rdf:about="https://purl.org/vir/IC5_Color">
        <rdfs:subClassOf rdf:resource="http://www.ics.forth.gr/isl/CRMsci/S9_Property_Type"/>
        <rdfs:comment>The class comprise concept coming from vocabularies and thesauri used to characterise the combination of a particular pigment (or set of pigments) with the reflected or transmitted light</rdfs:comment>
        <rdfs:label xml:lang="en">Color</rdfs:label>
    </owl:Class>
    


    <!-- https://purl.org/vir/IC8_Layer -->

    <owl:Class rdf:about="https://purl.org/vir/IC8_Layer">
        <rdfs:subClassOf rdf:resource="http://www.cidoc-crm.org/cidoc-crm/E25_Man-Made_Feature"/>
        <rdfs:comment>A layer is a stratum composed by one or more materials that cover a surface, or part of it, of a physical body. A Layer usually can rest on a physical object (wall), but can rest also on a previous layer</rdfs:comment>
        <rdfs:label xml:lang="en">Layer</rdfs:label>
    </owl:Class>
    


    <!-- https://purl.org/vir/IC9_Iconographical_Object -->

    <owl:Class rdf:about="https://purl.org/vir/IC9_Iconographical_Object">
        <rdfs:subClassOf rdf:resource="http://www.cidoc-crm.org/cidoc-crm/E36_Visual_Item"/>
        <rdfs:comment>A visual item that represent the nuclear characteristic of a particular set of symbols associate with a cognitive type of a person, animal or concept</rdfs:comment>
        <rdfs:label xml:lang="en">Iconographical Object</rdfs:label>
    </owl:Class>
</rdf:RDF>



<!-- Generated by the OWL API (version 4.5.2) https://github.com/owlcs/owlapi -->

